add no-trigger flag, some lemmas regarding release progress (broken)

src/algorithm_verified.ml
@@ -9,9 +9,53 @@ let no_mw = ref false
 module IntMap = Map.Make(struct type t = int let compare = Stdlib.compare end)
 open IntMap
 
+let rec string_of_term (t: Verified.Monitor.trm): string = begin match t with
+| Var n -> "Var"
+| Const c -> "Const"
+| Plus (t1, t2) -> "Plus (" ^ (string_of_term t1) ^ ") (" ^ (string_of_term t2) ^ ")"
+| Minus (t1, t2) -> "Minus (" ^ (string_of_term t1) ^ ") (" ^ (string_of_term t2) ^ ")"
+| UMinus t -> "UMinus (" ^ (string_of_term t) ^ ")"
+| Mult (t1, t2) -> "Mult (" ^ (string_of_term t1) ^ ") (" ^ (string_of_term t2) ^ ")"
+| Div (t1, t2) -> "Div (" ^ (string_of_term t1) ^ ") (" ^ (string_of_term t2) ^ ")"
+| Mod (t1, t2) -> "Mod (" ^ (string_of_term t1) ^ ") (" ^ (string_of_term t2) ^ ")"
+| F2i t -> "F2i (" ^ (string_of_term t) ^ ")"
+| I2f t -> "I2f (" ^ (string_of_term t) ^ ")"
+end
+
+let rec string_of_formula (f: Verified.Monitor.formula): string = begin match f with
+| Pred (s, trms) -> "Pred '" ^ s ^ "'"
+| Let (s, f1, f2) -> "Let " ^ s ^ " = (" ^ (string_of_formula f1) ^ ") in (" ^ (string_of_formula f2) ^")"
+| Eq (t1, t2) -> "Eq (" ^ (string_of_term t1) ^ ") (" ^ (string_of_term t2) ^ ")"
+| Less (t1, t2) -> "Less (" ^ (string_of_term t1) ^ ") (" ^ (string_of_term t2) ^ ")"
+| LessEq (t1, t2) -> "LessEq (" ^ (string_of_term t1) ^ ") (" ^ (string_of_term t2) ^ ")"
+| Neg f -> "Neg (" ^ (string_of_formula f) ^ ")"
+| Or (f1, f2) -> "Or (" ^ (string_of_formula f1) ^ ") I (" ^ (string_of_formula f2) ^ ")"
+| And (f1, f2) -> "And (" ^ (string_of_formula f1) ^ ") I (" ^ (string_of_formula f2) ^ ")"
+| Ands fs -> "Ands (" ^ (String.concat ", " (List.map string_of_formula fs)) ^ ")"
+| Exists f -> "Exists (" ^ (string_of_formula f) ^ ")"
+| Agg (n, agg, m, t, f) -> ""
+| Prev (i, f) -> "Prev I (" ^ (string_of_formula f) ^ ")"
+| Next (i, f) -> "Next I (" ^ (string_of_formula f) ^ ")"
+| Since (f1, i, f2) -> "Since (" ^ (string_of_formula f1) ^ ") I (" ^ (string_of_formula f2) ^ ")"
+| Until (f1, i, f2) -> "Until (" ^ (string_of_formula f1) ^ ") I (" ^ (string_of_formula f2) ^ ")"
+| Trigger (f1, i, f2) -> "Trigger (" ^ (string_of_formula f1) ^ ") I (" ^ (string_of_formula f2) ^ ")"
+| Release (f1, i, f2) -> "Release (" ^ (string_of_formula f1) ^ ") I (" ^ (string_of_formula f2) ^ ")"
+| MatchF (i, r) -> ""
+| MatchP (i, r) -> ""
+end
+
 let monitor dbschema logfile f =
   let closed = (free_vars f = []) in
   let cf = convert_formula dbschema f in
+  let _ = Printf.printf "%s\n" (string_of_formula cf); flush stdout in
+  let cf = if !Misc.no_trigger then Verified.Monitor.rewrite_trigger cf else cf in
+  let s = Verified.Monitor.mmonitorable_exec cf in
+  let _ = if s then
+	  (Printf.printf "ok\n"; flush stdout)
+	else
+	  (Printf.printf "not ok\n"; flush stdout)
+  in
+  let _ = Printf.printf "%s\n" (string_of_formula cf); flush stdout in
   let cf = if !no_mw then cf else Monitor.convert_multiway cf in
   let init_state = Monitor.minit_safe cf in
   let lexbuf = Log.log_open logfile in
