src/misc.mli
@@ -68,6 +68,7 @@ val stop_at_out_of_order_ts: bool ref
   (** Flags corresponding to the command-line options: -verbose, -check, -no_new_last_ts, -ignore_errors, -stop_at_out_of_order_ts. *)
 
 val no_rw: bool ref
+val no_trigger: bool ref
 val stop_at_first_viol: bool ref
 (** Flags corresponding to the command-line options -verbose,
     -check, -no_new_last_ts, -no_rw, and -stop_at_last_viol. *)
