src/verified.ml
@@ -300,6 +300,7 @@ module Monitor : sig
                               ((event_data option) list) set))))))))))),
         unit)
         mstate_ext
+  val rewrite_trigger : formula -> formula
 end = struct
 
 let ceq_funa : (('a -> 'b) -> ('a -> 'b) -> bool) option = None;;
@@ -2360,60 +2361,26 @@ let rec exhaustive_fusion
         not (proper_interval None (Some x)) &&
           exhaustive_above_fusion proper_interval g x sa);;
 
-let rec list_remdups
-  equal x1 = match equal, x1 with
-    equal, x :: xs ->
-      (if list_member equal xs x then list_remdups equal xs
-        else x :: list_remdups equal xs)
-    | equal, [] -> [];;
+let rec carda _A = carda _A;;
 
-let rec length _A xa = size_list (list_of_dlist _A xa);;
-
-let rec card (_A1, _A2, _A3)
-  = function
-    Complement a ->
-      (let aa = card (_A1, _A2, _A3) a in
-       let s = of_phantom (card_UNIV _A1) in
-        (if less_nat zero_nata s then minus_nata s aa
-          else (if finitea _A1.finite_UNIV_card_UNIV a then zero_nata
-                 else failwith "card Complement: infinite"
-                        (fun _ -> card (_A1, _A2, _A3) (Complement a)))))
-    | Set_Monad xs ->
-        (match ceq _A2
-          with None ->
-            failwith "card Set_Monad: ceq = None"
-              (fun _ -> card (_A1, _A2, _A3) (Set_Monad xs))
-          | Some eq -> size_list (list_remdups eq xs))
-    | RBT_set rbt ->
-        (match ccompare _A3
-          with None ->
-            failwith "card RBT_set: ccompare = None"
-              (fun _ -> card (_A1, _A2, _A3) (RBT_set rbt))
-          | Some _ -> size_list (keysb _A3 rbt))
-    | DList_set dxs ->
-        (match ceq _A2
-          with None ->
-            failwith "card DList_set: ceq = None"
-              (fun _ -> card (_A1, _A2, _A3) (DList_set dxs))
-          | Some _ -> length _A2 dxs);;
-
-let rec is_UNIV (_A1, _A2, _A3)
+let rec is_UNIV (_A1, _A2, _A3, _A4)
   = function
     RBT_set rbt ->
       (match ccompare _A3.ccompare_cproper_interval
         with None ->
           failwith "is_UNIV RBT_set: ccompare = None"
-            (fun _ -> is_UNIV (_A1, _A2, _A3) (RBT_set rbt))
+            (fun _ -> is_UNIV (_A1, _A2, _A3, _A4) (RBT_set rbt))
         | Some _ ->
           of_phantom (finite_UNIV _A1.finite_UNIV_card_UNIV) &&
             exhaustive_fusion (cproper_interval _A3) rbt_keys_generator
               (init _A3.ccompare_cproper_interval rbt))
-    | a -> (let aa = of_phantom (card_UNIV _A1) in
-            let b = card (_A1, _A2, _A3.ccompare_cproper_interval) a in
+    | a -> (let aa =
+              carda _A1 (top_set (_A2, _A3.ccompare_cproper_interval, _A4)) in
+            let b = carda _A1 a in
              (if less_nat zero_nata aa then equal_nata aa b
                else (if less_nat zero_nata b then false
                       else failwith "is_UNIV called on infinite type and set"
-                             (fun _ -> is_UNIV (_A1, _A2, _A3) a))));;
+                             (fun _ -> is_UNIV (_A1, _A2, _A3, _A4) a))));;
 
 let rec is_emptya _A
   xa = (match impl_ofa _A xa with Empty -> true
@@ -2421,19 +2388,19 @@ let rec is_emptya _A
 
 let rec nulla _A xa = null (list_of_dlist _A xa);;
 
-let rec is_empty (_A1, _A2, _A3)
-  = function Complement a -> is_UNIV (_A1, _A2, _A3) a
+let rec is_empty (_A1, _A2, _A3, _A4)
+  = function Complement a -> is_UNIV (_A1, _A2, _A3, _A4) a
     | RBT_set rbt ->
         (match ccompare _A3.ccompare_cproper_interval
           with None ->
             failwith "is_empty RBT_set: ccompare = None"
-              (fun _ -> is_empty (_A1, _A2, _A3) (RBT_set rbt))
+              (fun _ -> is_empty (_A1, _A2, _A3, _A4) (RBT_set rbt))
           | Some _ -> is_emptya _A3.ccompare_cproper_interval rbt)
     | DList_set dxs ->
         (match ceq _A2
           with None ->
             failwith "is_empty DList_set: ceq = None"
-              (fun _ -> is_empty (_A1, _A2, _A3) (DList_set dxs))
+              (fun _ -> is_empty (_A1, _A2, _A3, _A4) (DList_set dxs))
           | Some _ -> nulla _A2 dxs)
     | Set_Monad xs -> null xs;;
 
@@ -2537,8 +2504,8 @@ let rec cproper_interval_seta (_A1, _A2, _A3, _A4)
               proper_interval_set_aux (lt_of_comp c) (cproper_interval _A3)
                 (csorted_list_of_set (_A2, _A3.ccompare_cproper_interval) a)
                 (csorted_list_of_set (_A2, _A3.ccompare_cproper_interval) b))
-    | Some a, None -> not (is_UNIV (_A1, _A2, _A3) a)
-    | None, Some b -> not (is_empty (_A1, _A2, _A3) b)
+    | Some a, None -> not (is_UNIV (_A1, _A2, _A3, _A4) a)
+    | None, Some b -> not (is_empty (_A1, _A2, _A3, _A4) b)
     | None, None -> true;;
 
 let rec cproper_interval_set (_A1, _A2, _A3, _A4) =
@@ -4084,9 +4051,48 @@ let rec lookup _A xa = map_of _A (impl_of xa);;
 
 let rec updatea _A xc xd xe = Alist (update _A xc xd (impl_of xe));;
 
-let rec ecard (_A1, _A2, _A3)
+let rec list_remdups
+  equal x1 = match equal, x1 with
+    equal, x :: xs ->
+      (if list_member equal xs x then list_remdups equal xs
+        else x :: list_remdups equal xs)
+    | equal, [] -> [];;
+
+let rec length _A xa = size_list (list_of_dlist _A xa);;
+
+let rec card (_A1, _A2, _A3, _A4)
+  = function
+    Complement a ->
+      (let aa = carda _A1 a in
+       let s = carda _A1 (top_set (_A2, _A3, _A4)) in
+        (if less_nat zero_nata s then minus_nata s aa
+          else (if finitea _A1.finite_UNIV_card_UNIV a then zero_nata
+                 else failwith "card Complement: infinite"
+                        (fun _ -> carda _A1 (Complement a)))))
+    | Set_Monad xs ->
+        (match ceq _A2
+          with None ->
+            failwith "card Set_Monad: ceq = None"
+              (fun _ -> card (_A1, _A2, _A3, _A4) (Set_Monad xs))
+          | Some eq -> size_list (list_remdups eq xs))
+    | RBT_set rbt ->
+        (match ccompare _A3
+          with None ->
+            failwith "card RBT_set: ccompare = None"
+              (fun _ -> card (_A1, _A2, _A3, _A4) (RBT_set rbt))
+          | Some _ -> size_list (keysb _A3 rbt))
+    | DList_set dxs ->
+        (match ceq _A2
+          with None ->
+            failwith "card DList_set: ceq = None"
+              (fun _ -> card (_A1, _A2, _A3, _A4) (DList_set dxs))
+          | Some _ -> length _A2 dxs);;
+
+let rec ecard (_A1, _A2, _A3, _A4)
   a = (if finite (_A1.finite_UNIV_card_UNIV, _A2, _A3) a
-        then Enat (card (_A1, _A2, _A3) a) else Infinity_enat);;
+        then Enat (card (_A1, _A2, _A3, _A4) a) else Infinity_enat);;
+
+let first : formula = Neg (Prev (all, tt));;
 
 let rec rep_I (Abs_I x) = x;;
 
@@ -4424,7 +4430,8 @@ let rec eval_agg
   n g0 y omega b f rel =
     (if g0 && is_empty
                 (card_UNIV_list, (ceq_list (ceq_option ceq_event_data)),
-                  (cproper_interval_list (ccompare_option ccompare_event_data)))
+                  (cproper_interval_list (ccompare_option ccompare_event_data)),
+                  set_impl_list)
                 rel
       then singleton_table (ceq_event_data, ccompare_event_data) n y
              (eval_agg_op omega
@@ -4456,7 +4463,8 @@ let rec eval_agg
                       (ya, ecard (card_UNIV_list,
                                    (ceq_list (ceq_option ceq_event_data)),
                                    (ccompare_list
-                                     (ccompare_option ccompare_event_data)))
+                                     (ccompare_option ccompare_event_data)),
+                                   set_impl_list)
                              (filter
                                ((ceq_list (ceq_option ceq_event_data)),
                                  (ccompare_list
@@ -4524,7 +4532,7 @@ let rec safe_regex (_B1, _B2, _B3, _B4, _B5)
             safe_regex (_B1, _B2, _B3, _B4, _B5) fv safe Past Lax s)
     | fv, safe, m, g, Star r ->
         (equal_safety g Lax ||
-          is_empty (_B1, _B3, _B4)
+          is_empty (_B1, _B3, _B4, _B5)
             (fv_regex (_B3, _B4.ccompare_cproper_interval, _B5) fv r)) &&
           safe_regex (_B1, _B2, _B3, _B4, _B5) fv safe m g r;;
 
@@ -4652,6 +4660,38 @@ let rec r_delta (_A1, _A2, _A3)
     | kappa, x, phi_s, MStar r ->
         r_delta (_A1, _A2, _A3) (fun t -> kappa (MTimes (MStar r, t))) x phi_s
           r;;
+
+let rec int_remove_lower_bound
+  xa = Abs_I ((fun _ -> true), (memR xa, bounded xa));;
+
+let rec flip_int_less_lower
+  xa = Abs_I (if not (memL xa zero_nata)
+               then ((fun _ -> true), ((fun i -> not (memL xa i)), true))
+               else ((fun _ -> true), ((fun _ -> true), false)));;
+
+let rec eventually i phi = Until (tt, i, phi);;
+
+let rec always_safe_bounded
+  i phi =
+    And (eventually i phi,
+          Neg (eventually i
+                (And (Or (once (int_remove_lower_bound i) phi,
+                           eventually (int_remove_lower_bound i) phi),
+                       Neg phi))));;
+
+let rec release_safe_bounded
+  phi i psi =
+    And (eventually i tt,
+          Or (Or (always_safe_bounded i psi,
+                   eventually (flip_int_less_lower i) phi),
+               eventually (flip_int_less_lower i)
+                 (Next (all, Until (psi, int_remove_lower_bound i,
+                                     And (psi, phi))))));;
+
+let rec and_release_safe_bounded
+  phia phi i psi =
+    Or (And (phia, Neg (eventually i tt)),
+         And (phia, release_safe_bounded phi i psi));;
 
 let rec subset (_A1, _A2, _A3, _A4) = subset_eq (_A2, _A3, _A4);;
 
@@ -4914,147 +4954,147 @@ let rec safe_formula
           (fvi zero_nata phi) &&
           (safe_formula phi && safe_formula psi)
     | Neg (Pred (v, va)) ->
-        is_empty (card_UNIV_nat, ceq_nat, cproper_interval_nat)
+        is_empty (card_UNIV_nat, ceq_nat, cproper_interval_nat, set_impl_nat)
           (fvi zero_nata (Pred (v, va))) &&
           safe_formula (Pred (v, va))
     | Neg (Let (v, va, vb)) ->
-        is_empty (card_UNIV_nat, ceq_nat, cproper_interval_nat)
+        is_empty (card_UNIV_nat, ceq_nat, cproper_interval_nat, set_impl_nat)
           (fvi zero_nata (Let (v, va, vb))) &&
           safe_formula (Let (v, va, vb))
     | Neg (Eq (Const vb, va)) ->
-        is_empty (card_UNIV_nat, ceq_nat, cproper_interval_nat)
+        is_empty (card_UNIV_nat, ceq_nat, cproper_interval_nat, set_impl_nat)
           (fvi zero_nata (Eq (Const vb, va))) &&
           safe_formula (Eq (Const vb, va))
     | Neg (Eq (Plus (vb, vc), va)) ->
-        is_empty (card_UNIV_nat, ceq_nat, cproper_interval_nat)
+        is_empty (card_UNIV_nat, ceq_nat, cproper_interval_nat, set_impl_nat)
           (fvi zero_nata (Eq (Plus (vb, vc), va))) &&
           safe_formula (Eq (Plus (vb, vc), va))
     | Neg (Eq (Minus (vb, vc), va)) ->
-        is_empty (card_UNIV_nat, ceq_nat, cproper_interval_nat)
+        is_empty (card_UNIV_nat, ceq_nat, cproper_interval_nat, set_impl_nat)
           (fvi zero_nata (Eq (Minus (vb, vc), va))) &&
           safe_formula (Eq (Minus (vb, vc), va))
     | Neg (Eq (UMinus vb, va)) ->
-        is_empty (card_UNIV_nat, ceq_nat, cproper_interval_nat)
+        is_empty (card_UNIV_nat, ceq_nat, cproper_interval_nat, set_impl_nat)
           (fvi zero_nata (Eq (UMinus vb, va))) &&
           safe_formula (Eq (UMinus vb, va))
     | Neg (Eq (Mult (vb, vc), va)) ->
-        is_empty (card_UNIV_nat, ceq_nat, cproper_interval_nat)
+        is_empty (card_UNIV_nat, ceq_nat, cproper_interval_nat, set_impl_nat)
           (fvi zero_nata (Eq (Mult (vb, vc), va))) &&
           safe_formula (Eq (Mult (vb, vc), va))
     | Neg (Eq (Div (vb, vc), va)) ->
-        is_empty (card_UNIV_nat, ceq_nat, cproper_interval_nat)
+        is_empty (card_UNIV_nat, ceq_nat, cproper_interval_nat, set_impl_nat)
           (fvi zero_nata (Eq (Div (vb, vc), va))) &&
           safe_formula (Eq (Div (vb, vc), va))
     | Neg (Eq (Mod (vb, vc), va)) ->
-        is_empty (card_UNIV_nat, ceq_nat, cproper_interval_nat)
+        is_empty (card_UNIV_nat, ceq_nat, cproper_interval_nat, set_impl_nat)
           (fvi zero_nata (Eq (Mod (vb, vc), va))) &&
           safe_formula (Eq (Mod (vb, vc), va))
     | Neg (Eq (F2i vb, va)) ->
-        is_empty (card_UNIV_nat, ceq_nat, cproper_interval_nat)
+        is_empty (card_UNIV_nat, ceq_nat, cproper_interval_nat, set_impl_nat)
           (fvi zero_nata (Eq (F2i vb, va))) &&
           safe_formula (Eq (F2i vb, va))
     | Neg (Eq (I2f vb, va)) ->
-        is_empty (card_UNIV_nat, ceq_nat, cproper_interval_nat)
+        is_empty (card_UNIV_nat, ceq_nat, cproper_interval_nat, set_impl_nat)
           (fvi zero_nata (Eq (I2f vb, va))) &&
           safe_formula (Eq (I2f vb, va))
     | Neg (Eq (v, Const vb)) ->
-        is_empty (card_UNIV_nat, ceq_nat, cproper_interval_nat)
+        is_empty (card_UNIV_nat, ceq_nat, cproper_interval_nat, set_impl_nat)
           (fvi zero_nata (Eq (v, Const vb))) &&
           safe_formula (Eq (v, Const vb))
     | Neg (Eq (v, Plus (vb, vc))) ->
-        is_empty (card_UNIV_nat, ceq_nat, cproper_interval_nat)
+        is_empty (card_UNIV_nat, ceq_nat, cproper_interval_nat, set_impl_nat)
           (fvi zero_nata (Eq (v, Plus (vb, vc)))) &&
           safe_formula (Eq (v, Plus (vb, vc)))
     | Neg (Eq (v, Minus (vb, vc))) ->
-        is_empty (card_UNIV_nat, ceq_nat, cproper_interval_nat)
+        is_empty (card_UNIV_nat, ceq_nat, cproper_interval_nat, set_impl_nat)
           (fvi zero_nata (Eq (v, Minus (vb, vc)))) &&
           safe_formula (Eq (v, Minus (vb, vc)))
     | Neg (Eq (v, UMinus vb)) ->
-        is_empty (card_UNIV_nat, ceq_nat, cproper_interval_nat)
+        is_empty (card_UNIV_nat, ceq_nat, cproper_interval_nat, set_impl_nat)
           (fvi zero_nata (Eq (v, UMinus vb))) &&
           safe_formula (Eq (v, UMinus vb))
     | Neg (Eq (v, Mult (vb, vc))) ->
-        is_empty (card_UNIV_nat, ceq_nat, cproper_interval_nat)
+        is_empty (card_UNIV_nat, ceq_nat, cproper_interval_nat, set_impl_nat)
           (fvi zero_nata (Eq (v, Mult (vb, vc)))) &&
           safe_formula (Eq (v, Mult (vb, vc)))
     | Neg (Eq (v, Div (vb, vc))) ->
-        is_empty (card_UNIV_nat, ceq_nat, cproper_interval_nat)
+        is_empty (card_UNIV_nat, ceq_nat, cproper_interval_nat, set_impl_nat)
           (fvi zero_nata (Eq (v, Div (vb, vc)))) &&
           safe_formula (Eq (v, Div (vb, vc)))
     | Neg (Eq (v, Mod (vb, vc))) ->
-        is_empty (card_UNIV_nat, ceq_nat, cproper_interval_nat)
+        is_empty (card_UNIV_nat, ceq_nat, cproper_interval_nat, set_impl_nat)
           (fvi zero_nata (Eq (v, Mod (vb, vc)))) &&
           safe_formula (Eq (v, Mod (vb, vc)))
     | Neg (Eq (v, F2i vb)) ->
-        is_empty (card_UNIV_nat, ceq_nat, cproper_interval_nat)
+        is_empty (card_UNIV_nat, ceq_nat, cproper_interval_nat, set_impl_nat)
           (fvi zero_nata (Eq (v, F2i vb))) &&
           safe_formula (Eq (v, F2i vb))
     | Neg (Eq (v, I2f vb)) ->
-        is_empty (card_UNIV_nat, ceq_nat, cproper_interval_nat)
+        is_empty (card_UNIV_nat, ceq_nat, cproper_interval_nat, set_impl_nat)
           (fvi zero_nata (Eq (v, I2f vb))) &&
           safe_formula (Eq (v, I2f vb))
     | Neg (Less (v, va)) ->
-        is_empty (card_UNIV_nat, ceq_nat, cproper_interval_nat)
+        is_empty (card_UNIV_nat, ceq_nat, cproper_interval_nat, set_impl_nat)
           (fvi zero_nata (Less (v, va))) &&
           safe_formula (Less (v, va))
     | Neg (LessEq (v, va)) ->
-        is_empty (card_UNIV_nat, ceq_nat, cproper_interval_nat)
+        is_empty (card_UNIV_nat, ceq_nat, cproper_interval_nat, set_impl_nat)
           (fvi zero_nata (LessEq (v, va))) &&
           safe_formula (LessEq (v, va))
     | Neg (Neg v) ->
-        is_empty (card_UNIV_nat, ceq_nat, cproper_interval_nat)
+        is_empty (card_UNIV_nat, ceq_nat, cproper_interval_nat, set_impl_nat)
           (fvi zero_nata (Neg v)) &&
           safe_formula (Neg v)
     | Neg (Or (v, va)) ->
-        is_empty (card_UNIV_nat, ceq_nat, cproper_interval_nat)
+        is_empty (card_UNIV_nat, ceq_nat, cproper_interval_nat, set_impl_nat)
           (fvi zero_nata (Or (v, va))) &&
           safe_formula (Or (v, va))
     | Neg (And (v, va)) ->
-        is_empty (card_UNIV_nat, ceq_nat, cproper_interval_nat)
+        is_empty (card_UNIV_nat, ceq_nat, cproper_interval_nat, set_impl_nat)
           (fvi zero_nata (And (v, va))) &&
           safe_formula (And (v, va))
     | Neg (Ands v) ->
-        is_empty (card_UNIV_nat, ceq_nat, cproper_interval_nat)
+        is_empty (card_UNIV_nat, ceq_nat, cproper_interval_nat, set_impl_nat)
           (fvi zero_nata (Ands v)) &&
           safe_formula (Ands v)
     | Neg (Exists v) ->
-        is_empty (card_UNIV_nat, ceq_nat, cproper_interval_nat)
+        is_empty (card_UNIV_nat, ceq_nat, cproper_interval_nat, set_impl_nat)
           (fvi zero_nata (Exists v)) &&
           safe_formula (Exists v)
     | Neg (Agg (v, va, vb, vc, vd)) ->
-        is_empty (card_UNIV_nat, ceq_nat, cproper_interval_nat)
+        is_empty (card_UNIV_nat, ceq_nat, cproper_interval_nat, set_impl_nat)
           (fvi zero_nata (Agg (v, va, vb, vc, vd))) &&
           safe_formula (Agg (v, va, vb, vc, vd))
     | Neg (Prev (v, va)) ->
-        is_empty (card_UNIV_nat, ceq_nat, cproper_interval_nat)
+        is_empty (card_UNIV_nat, ceq_nat, cproper_interval_nat, set_impl_nat)
           (fvi zero_nata (Prev (v, va))) &&
           safe_formula (Prev (v, va))
     | Neg (Next (v, va)) ->
-        is_empty (card_UNIV_nat, ceq_nat, cproper_interval_nat)
+        is_empty (card_UNIV_nat, ceq_nat, cproper_interval_nat, set_impl_nat)
           (fvi zero_nata (Next (v, va))) &&
           safe_formula (Next (v, va))
     | Neg (Since (v, va, vb)) ->
-        is_empty (card_UNIV_nat, ceq_nat, cproper_interval_nat)
+        is_empty (card_UNIV_nat, ceq_nat, cproper_interval_nat, set_impl_nat)
           (fvi zero_nata (Since (v, va, vb))) &&
           safe_formula (Since (v, va, vb))
     | Neg (Until (v, va, vb)) ->
-        is_empty (card_UNIV_nat, ceq_nat, cproper_interval_nat)
+        is_empty (card_UNIV_nat, ceq_nat, cproper_interval_nat, set_impl_nat)
           (fvi zero_nata (Until (v, va, vb))) &&
           safe_formula (Until (v, va, vb))
     | Neg (Trigger (v, va, vb)) ->
-        is_empty (card_UNIV_nat, ceq_nat, cproper_interval_nat)
+        is_empty (card_UNIV_nat, ceq_nat, cproper_interval_nat, set_impl_nat)
           (fvi zero_nata (Trigger (v, va, vb))) &&
           safe_formula (Trigger (v, va, vb))
     | Neg (Release (v, va, vb)) ->
-        is_empty (card_UNIV_nat, ceq_nat, cproper_interval_nat)
+        is_empty (card_UNIV_nat, ceq_nat, cproper_interval_nat, set_impl_nat)
           (fvi zero_nata (Release (v, va, vb))) &&
           safe_formula (Release (v, va, vb))
     | Neg (MatchF (v, va)) ->
-        is_empty (card_UNIV_nat, ceq_nat, cproper_interval_nat)
+        is_empty (card_UNIV_nat, ceq_nat, cproper_interval_nat, set_impl_nat)
           (fvi zero_nata (MatchF (v, va))) &&
           safe_formula (MatchF (v, va))
     | Neg (MatchP (v, va)) ->
-        is_empty (card_UNIV_nat, ceq_nat, cproper_interval_nat)
+        is_empty (card_UNIV_nat, ceq_nat, cproper_interval_nat, set_impl_nat)
           (fvi zero_nata (MatchP (v, va))) &&
           safe_formula (MatchP (v, va))
     | Or (phi, psi) ->
@@ -5077,8 +5117,18 @@ let rec safe_formula
                     | Since (_, _, _) -> false | Until (_, _, _) -> false
                     | Trigger (a, b, c) ->
                       safe_formula_dual true safe_formula a b c
-                    | Release (_, _, _) -> false | MatchF (_, _) -> false
-                    | MatchP (_, _) -> false))))
+                    | Release (phia, i, psia) ->
+                      bounded i &&
+                        (not (memL i zero_nata && memR i zero_nata) &&
+                          (safe_formula phia &&
+                            (safe_formula psia &&
+                              (eq_set
+                                 (card_UNIV_nat, cenum_nat, ceq_nat,
+                                   ccompare_nat)
+                                 (fvi zero_nata phia) (fvi zero_nata psia) &&
+                                safe_formula
+                                  (and_release_safe_bounded phi phia i psia)))))
+                    | MatchF (_, _) -> false | MatchP (_, _) -> false))))
     | Ands l ->
         (let (pos, neg) = partition safe_formula l in
           not (null pos) &&
@@ -5249,8 +5299,6 @@ let rec to_mregex_exec
 
 let rec to_mregex r = to_mregex_exec r [];;
 
-let rec eventually i phi = Until (tt, i, phi);;
-
 let rec remove_neg = function Neg phi -> phi
                      | Pred (v, va) -> Pred (v, va)
                      | Let (v, va, vb) -> Let (v, va, vb)
@@ -5325,11 +5373,7 @@ let rec score (_A1, _A2)
                   (finite_UNIV_list, (ceq_list (ceq_option _A1)),
                     (cproper_interval_list (ccompare_option _A2)),
                     set_impl_list))))
-          comm_monoid_add_nat
-          (fun (_, a) ->
-            card (card_UNIV_list, (ceq_list (ceq_option _A1)),
-                   (ccompare_list (ccompare_option _A2)))
-              a)
+          comm_monoid_add_nat (fun (_, a) -> carda card_UNIV_list a)
           (filter
             ((ceq_prod
                (ceq_set
@@ -5414,7 +5458,8 @@ let rec mrtabulate (_A1, _A2)
                 (let fk = f k in
                   (if is_empty
                         (card_UNIV_list, (ceq_list (ceq_option _A1)),
-                          (cproper_interval_list (ccompare_option _A2)))
+                          (cproper_interval_list (ccompare_option _A2)),
+                          set_impl_list)
                         fk
                     then None else Some (k, fk))))
               xs)));;
@@ -5901,11 +5946,6 @@ let rec takedropWhile_queue
               then (let (qb, asa) = takedropWhile_queue f (tl_queue qa) in
                      (qb, a :: asa))
               else (qa, [])));;
-
-let rec flip_int_less_lower
-  xa = Abs_I (if not (memL xa zero_nata)
-               then ((fun _ -> true), ((fun i -> not (memL xa i)), true))
-               else ((fun _ -> true), ((fun _ -> true), false)));;
 
 let rec dropWhile_queue
   f q = (match safe_hd q with (None, qa) -> qa
@@ -6444,7 +6484,8 @@ let rec filterQuery (_A1, _A2)
                   (cproper_interval_list (ccompare_option _A2)),
                   set_impl_list))))
           (fun (s, _) ->
-            not (is_empty (card_UNIV_nat, ceq_nat, cproper_interval_nat)
+            not (is_empty
+                  (card_UNIV_nat, ceq_nat, cproper_interval_nat, set_impl_nat)
                   (inf_seta (ceq_nat, ccompare_nat) s v)))
           q;;
 
@@ -6522,7 +6563,8 @@ let rec max_getIJ (_A1, _A2)
                 (cproper_interval_set
                   (card_UNIV_list, (ceq_list (ceq_option _A1)),
                     (cproper_interval_list (ccompare_option _A2)),
-                    set_impl_list))))
+                    set_impl_list))),
+              (set_impl_prod set_impl_set set_impl_set))
             q_neg
         then (let x = arg_max_list linorder_nat (score (_A1, _A2) q_pos) l in
                (insert (ceq_nat, ccompare_nat) x
@@ -6543,7 +6585,7 @@ let rec max_getIJ (_A1, _A2)
 
 let rec new_max_getIJ_genericJoin (_A1, _A2)
   v q_pos q_neg =
-    (if less_eq_nat (card (card_UNIV_nat, ceq_nat, ccompare_nat) v) one_nata
+    (if less_eq_nat (carda card_UNIV_nat v) one_nata
       then remove_Union
              (finite_UNIV_list, cenum_list, (ceq_list (ceq_option _A1)),
                (cproper_interval_list (ccompare_option _A2)), set_impl_list)
@@ -6603,7 +6645,8 @@ let rec new_max_getIJ_genericJoin (_A1, _A2)
             let r_I = new_max_getIJ_genericJoin (_A1, _A2) i q_I_pos q_I_neg in
              (if is_empty
                    (card_UNIV_list, (ceq_list (ceq_option _A1)),
-                     (cproper_interval_list (ccompare_option _A2)))
+                     (cproper_interval_list (ccompare_option _A2)),
+                     set_impl_list)
                    r_I
                then set_empty
                       ((ceq_list (ceq_option _A1)),
@@ -6828,7 +6871,7 @@ let rec new_max_getIJ_wrapperGenericJoin (_A1, _A2)
           (fun (_, a) ->
             is_empty
               (card_UNIV_list, (ceq_list (ceq_option _A1)),
-                (cproper_interval_list (ccompare_option _A2)))
+                (cproper_interval_list (ccompare_option _A2)), set_impl_list)
               a) ||
           bex ((ceq_prod
                  (ceq_set
@@ -6848,10 +6891,13 @@ let rec new_max_getIJ_wrapperGenericJoin (_A1, _A2)
                       set_impl_list))))
             q_neg
             (fun (a, x) ->
-              is_empty (card_UNIV_nat, ceq_nat, cproper_interval_nat) a &&
+              is_empty
+                (card_UNIV_nat, ceq_nat, cproper_interval_nat, set_impl_nat)
+                a &&
                 not (is_empty
                       (card_UNIV_list, (ceq_list (ceq_option _A1)),
-                        (cproper_interval_list (ccompare_option _A2)))
+                        (cproper_interval_list (ccompare_option _A2)),
+                        set_impl_list)
                       x))
       then set_empty
              ((ceq_list (ceq_option _A1)),
@@ -6876,7 +6922,9 @@ let rec new_max_getIJ_wrapperGenericJoin (_A1, _A2)
                         (cproper_interval_list (ccompare_option _A2)),
                         set_impl_list))))
                 (fun (a, _) ->
-                  not (is_empty (card_UNIV_nat, ceq_nat, cproper_interval_nat)
+                  not (is_empty
+                        (card_UNIV_nat, ceq_nat, cproper_interval_nat,
+                          set_impl_nat)
                         a))
                 q_pos
               in
@@ -6899,7 +6947,8 @@ let rec new_max_getIJ_wrapperGenericJoin (_A1, _A2)
                        (cproper_interval_set
                          (card_UNIV_list, (ceq_list (ceq_option _A1)),
                            (cproper_interval_list (ccompare_option _A2)),
-                           set_impl_list))))
+                           set_impl_list))),
+                     (set_impl_prod set_impl_set set_impl_set))
                    q
                then remove_Union
                       (finite_UNIV_list, cenum_list,
@@ -7015,8 +7064,7 @@ let rec new_max_getIJ_wrapperGenericJoin (_A1, _A2)
                            subset
                              (card_UNIV_nat, cenum_nat, ceq_nat, ccompare_nat) a
                              v &&
-                             less_eq_nat one_nata
-                               (card (card_UNIV_nat, ceq_nat, ccompare_nat) a))
+                             less_eq_nat one_nata (carda card_UNIV_nat a))
                          q_neg
                        in
                       new_max_getIJ_genericJoin (_A1, _A2) v q a))));;
@@ -7068,9 +7116,10 @@ let rec join_mask
 
 let rec remove_cfi (_A1, _A2) = Abs_comp_fun_idem (remove (_A1, _A2));;
 
-let rec set_minus (_A1, _A2, _A3)
+let rec set_minus (_A1, _A2, _A3, _A4)
   x y = (if finite (_A1.finite_UNIV_card_UNIV, _A2, _A3) y &&
-              less_nat (card (_A1, _A2, _A3) y) (card (_A1, _A2, _A3) x)
+              less_nat (card (_A1, _A2, _A3, _A4) y)
+                (card (_A1, _A2, _A3, _A4) x)
           then set_fold_cfi (_A2, _A3) (remove_cfi (_A2, _A3)) x y
           else minus_set (_A2, _A3) x y);;
 
@@ -7078,7 +7127,7 @@ let rec bin_join (_A1, _A2, _A3)
   n aa ta pos a t =
     (if is_empty
           (card_UNIV_list, (ceq_list (ceq_option _A1)),
-            (cproper_interval_list (ccompare_option _A2)))
+            (cproper_interval_list (ccompare_option _A2)), set_impl_list)
           ta
       then set_empty
              ((ceq_list (ceq_option _A1)),
@@ -7086,7 +7135,7 @@ let rec bin_join (_A1, _A2, _A3)
              (of_phantom set_impl_lista)
       else (if is_empty
                  (card_UNIV_list, (ceq_list (ceq_option _A1)),
-                   (cproper_interval_list (ccompare_option _A2)))
+                   (cproper_interval_list (ccompare_option _A2)), set_impl_list)
                  t
              then (if pos
                     then set_empty
@@ -7094,7 +7143,10 @@ let rec bin_join (_A1, _A2, _A3)
                              (ccompare_list (ccompare_option _A2)))
                            (of_phantom set_impl_lista)
                     else ta)
-             else (if is_empty (card_UNIV_nat, ceq_nat, cproper_interval_nat) a
+             else (if is_empty
+                        (card_UNIV_nat, ceq_nat, cproper_interval_nat,
+                          set_impl_nat)
+                        a
                     then (if equal_boola pos
                                (member
                                  ((ceq_list (ceq_option _A1)),
@@ -7113,7 +7165,7 @@ let rec bin_join (_A1, _A2, _A3)
  ((ceq_list (ceq_option _A1)), (ccompare_list (ccompare_option _A2))) ta t
                                   else set_minus
  (card_UNIV_list, (ceq_list (ceq_option _A1)),
-   (ccompare_list (ccompare_option _A2)))
+   (ccompare_list (ccompare_option _A2)), set_impl_list)
  ta t)
                            else (if subset
                                       (card_UNIV_nat, cenum_nat, ceq_nat,
@@ -7254,11 +7306,11 @@ let rec add_new_ts_mmsaux (_A1, _A2, _A3)
 
 let rec filter_not_in_cfi (_A1, _A2) = Abs_comp_fun_idem (deletea (_A1, _A2));;
 
-let rec filter_join (_A1, _A2, _A3, _A4)
+let rec filter_join (_A1, _A2, _A3, _A4, _A5)
   pos a m =
     (if not pos &&
           (finite (_A1.finite_UNIV_card_UNIV, _A2, _A3) a &&
-            less_nat (card (_A1, _A2, _A3) a) (size _A3 m))
+            less_nat (card (_A1, _A2, _A3, _A5) a) (size _A3 m))
       then set_fold_cfi (_A2, _A3) (filter_not_in_cfi (_A3, _A4)) m a
       else filterb _A3
              (fun asa _ ->
@@ -7275,14 +7327,14 @@ let rec join_mmsaux (_A1, _A2, _A3)
                   filter_join
                     (card_UNIV_list, (ceq_list (ceq_option _A1)),
                       (ccompare_list (ccompare_option _A2)),
-                      (equal_list (equal_option _A3)))
+                      (equal_list (equal_option _A3)), set_impl_list)
                     pos x tuple_in
                   in
                 let tuple_sincea =
                   filter_join
                     (card_UNIV_list, (ceq_list (ceq_option _A1)),
                       (ccompare_list (ccompare_option _A2)),
-                      (equal_list (equal_option _A3)))
+                      (equal_list (equal_option _A3)), set_impl_list)
                     pos x tuple_since
                   in
                  (t, (gc, (maskL,
@@ -7477,7 +7529,7 @@ let rec r_epsilon_strict (_A1, _A2, _A3)
     | n, phi_s, MTestNeg i ->
         (if is_empty
               (card_UNIV_list, (ceq_list (ceq_option _A1)),
-                (cproper_interval_list (ccompare_option _A2)))
+                (cproper_interval_list (ccompare_option _A2)), set_impl_list)
               (nth phi_s i)
           then unit_table (_A1, _A2) n
           else empty_table
@@ -7580,7 +7632,7 @@ let rec l_epsilon_strict (_A1, _A2, _A3)
     | n, phi_s, MTestNeg i ->
         (if is_empty
               (card_UNIV_list, (ceq_list (ceq_option _A1)),
-                (cproper_interval_list (ccompare_option _A2)))
+                (cproper_interval_list (ccompare_option _A2)), set_impl_list)
               (nth phi_s i)
           then unit_table (_A1, _A2) n
           else empty_table
@@ -7776,7 +7828,8 @@ let rec meval
                   (if is_empty
                         (card_UNIV_list, (ceq_list (ceq_option ceq_event_data)),
                           (cproper_interval_list
-                            (ccompare_option ccompare_event_data)))
+                            (ccompare_option ccompare_event_data)),
+                          set_impl_list)
                         r
                     then unit_table (ceq_event_data, ccompare_event_data) n
                     else empty_table
@@ -7803,9 +7856,12 @@ let rec meval
          let (zs, bufb) =
            mbufn_take
              (fun xs zs ->
-               zs @ [mmulti_join
+               let r = (zs @ [let _ = Printf.printf "start mmultijoin\n"; flush stdout in mmulti_join
                        (ceq_event_data, ccompare_event_data, equal_event_data) n
-                       a_pos a_neg xs])
+				   a_pos a_neg xs]) in
+					   let _ = Printf.printf "done mmultijoin\n"; in
+					   r
+				   )
              [] buf
            in
           (zs, MAnds (a_pos, a_neg, mapa snd r, bufb)))
@@ -7931,26 +7987,6 @@ let rec meval
                a),
           MPred (e, tms))
     | n, ts, db, MRel rel -> (replicate (size_list ts) rel, MRel rel);;
-
-let rec int_remove_lower_bound
-  xa = Abs_I ((fun _ -> true), (memR xa, bounded xa));;
-
-let rec always_safe_bounded
-  i phi =
-    And (eventually i phi,
-          Neg (eventually i
-                (And (Or (once (int_remove_lower_bound i) phi,
-                           eventually (int_remove_lower_bound i) phi),
-                       Neg phi))));;
-
-let rec release_safe_bounded
-  phi i psi =
-    And (eventually i tt,
-          Or (Or (always_safe_bounded i psi,
-                   eventually (flip_int_less_lower i) phi),
-               eventually (flip_int_less_lower i)
-                 (Next (all, Until (psi, int_remove_lower_bound i,
-                                     And (psi, phi))))));;
 
 let mapping_impl_nat : (nat, mapping_impla) phantom = Phantom Mapping_RBT;;
 
@@ -8094,7 +8130,8 @@ let rec minit0
   n x1 = match n, x1 with
     n, Neg phi ->
       (let v = fvi zero_nata phi in
-        (if is_empty (card_UNIV_nat, ceq_nat, cproper_interval_nat) v
+        (if is_empty
+              (card_UNIV_nat, ceq_nat, cproper_interval_nat, set_impl_nat) v
           then MNeg (minit0 n phi)
           else MRel (empty_table
                       ((ceq_list (ceq_option ceq_event_data)),
@@ -8132,7 +8169,11 @@ fvi zero_nata psia, minit0 n psia, ([], []))
       init_args i n (fvi zero_nata phiaa) (fvi zero_nata psia) false,
       minit0 n phiaa, minit0 n psia, ([], []), [],
       init_mmtaux (ceq_event_data, ccompare_event_data)
-        (init_args i n (fvi zero_nata phiaa) (fvi zero_nata psia) false))))))))
+        (init_args i n (fvi zero_nata phiaa) (fvi zero_nata psia) false))))
+                               | Release (phia, i, psia) ->
+                                 minit0 n
+                                   (and_release_safe_bounded phi phia i
+                                     psia)))))
     | n, Ands l ->
         (let (pos, neg) = partition safe_formula l in
          let mpos = mapa (minit0 n) pos in
@@ -8229,7 +8270,7 @@ let rec mk_db
           (fun (p, x) ->
             (if is_empty
                   (card_UNIV_list, (ceq_list ceq_event_data),
-                    (cproper_interval_list ccompare_event_data))
+                    (cproper_interval_list ccompare_event_data), set_impl_list)
                   x
               then None else Some (p, [x])))
           (clearjunk equal_string8 t));;
@@ -8470,7 +8511,8 @@ let rec vmeval
                   (if is_empty
                         (card_UNIV_list, (ceq_list (ceq_option ceq_event_data)),
                           (cproper_interval_list
-                            (ccompare_option ccompare_event_data)))
+                            (ccompare_option ccompare_event_data)),
+                          set_impl_list)
                         r
                     then unit_table (ceq_event_data, ccompare_event_data) n
                     else empty_table
@@ -8597,7 +8639,8 @@ let rec vminit0
   n x1 = match n, x1 with
     n, Neg phi ->
       (let v = fvi zero_nata phi in
-        (if is_empty (card_UNIV_nat, ceq_nat, cproper_interval_nat) v
+        (if is_empty
+              (card_UNIV_nat, ceq_nat, cproper_interval_nat, set_impl_nat) v
           then MNeg (vminit0 n phi)
           else MRel (empty_table
                       ((ceq_list (ceq_option ceq_event_data)),
@@ -8635,7 +8678,11 @@ fvi zero_nata psia, vminit0 n psia, ([], []))
       init_args i n (fvi zero_nata phiaa) (fvi zero_nata psia) false,
       vminit0 n phiaa, vminit0 n psia, ([], []), [],
       init_mmtaux (ceq_event_data, ccompare_event_data)
-        (init_args i n (fvi zero_nata phiaa) (fvi zero_nata psia) false))))))))
+        (init_args i n (fvi zero_nata phiaa) (fvi zero_nata psia) false))))
+                               | Release (phia, i, psia) ->
+                                 vminit0 n
+                                   (and_release_safe_bounded phi phia i
+                                     psia)))))
     | n, Ands l ->
         (let (pos, neg) = partition safe_formula l in
          let mpos = mapa (vminit0 n) pos in
@@ -8767,6 +8814,16 @@ let rec map_regex
     | f, Times (x41, x42) -> Times (map_regex f x41, map_regex f x42)
     | f, Star x5 -> Star (map_regex f x5);;
 
+let rec historically_safe_0
+  i phi =
+    (if bounded i
+      then Or (Since (phi, flip_int i, Next (all, phi)),
+                Since (phi, i, And (first, phi)))
+      else Since (phi, i, And (first, phi)));;
+
+let rec trigger_safe_0
+  phi i psi = Or (Since (psi, i, And (psi, phi)), historically_safe_0 i psi);;
+
 let rbt_empty : ((event_data list), unit) mapping_rbt
   = emptyc (ccompare_list ccompare_event_data);;
 
@@ -8780,147 +8837,147 @@ let rec mmonitorable_exec
           (fvi zero_nata phi) &&
           (mmonitorable_exec phi && mmonitorable_exec psi)
     | Neg (Pred (v, va)) ->
-        is_empty (card_UNIV_nat, ceq_nat, cproper_interval_nat)
+        is_empty (card_UNIV_nat, ceq_nat, cproper_interval_nat, set_impl_nat)
           (fvi zero_nata (Pred (v, va))) &&
           mmonitorable_exec (Pred (v, va))
     | Neg (Let (v, va, vb)) ->
-        is_empty (card_UNIV_nat, ceq_nat, cproper_interval_nat)
+        is_empty (card_UNIV_nat, ceq_nat, cproper_interval_nat, set_impl_nat)
           (fvi zero_nata (Let (v, va, vb))) &&
           mmonitorable_exec (Let (v, va, vb))
     | Neg (Eq (Const vb, va)) ->
-        is_empty (card_UNIV_nat, ceq_nat, cproper_interval_nat)
+        is_empty (card_UNIV_nat, ceq_nat, cproper_interval_nat, set_impl_nat)
           (fvi zero_nata (Eq (Const vb, va))) &&
           mmonitorable_exec (Eq (Const vb, va))
     | Neg (Eq (Plus (vb, vc), va)) ->
-        is_empty (card_UNIV_nat, ceq_nat, cproper_interval_nat)
+        is_empty (card_UNIV_nat, ceq_nat, cproper_interval_nat, set_impl_nat)
           (fvi zero_nata (Eq (Plus (vb, vc), va))) &&
           mmonitorable_exec (Eq (Plus (vb, vc), va))
     | Neg (Eq (Minus (vb, vc), va)) ->
-        is_empty (card_UNIV_nat, ceq_nat, cproper_interval_nat)
+        is_empty (card_UNIV_nat, ceq_nat, cproper_interval_nat, set_impl_nat)
           (fvi zero_nata (Eq (Minus (vb, vc), va))) &&
           mmonitorable_exec (Eq (Minus (vb, vc), va))
     | Neg (Eq (UMinus vb, va)) ->
-        is_empty (card_UNIV_nat, ceq_nat, cproper_interval_nat)
+        is_empty (card_UNIV_nat, ceq_nat, cproper_interval_nat, set_impl_nat)
           (fvi zero_nata (Eq (UMinus vb, va))) &&
           mmonitorable_exec (Eq (UMinus vb, va))
     | Neg (Eq (Mult (vb, vc), va)) ->
-        is_empty (card_UNIV_nat, ceq_nat, cproper_interval_nat)
+        is_empty (card_UNIV_nat, ceq_nat, cproper_interval_nat, set_impl_nat)
           (fvi zero_nata (Eq (Mult (vb, vc), va))) &&
           mmonitorable_exec (Eq (Mult (vb, vc), va))
     | Neg (Eq (Div (vb, vc), va)) ->
-        is_empty (card_UNIV_nat, ceq_nat, cproper_interval_nat)
+        is_empty (card_UNIV_nat, ceq_nat, cproper_interval_nat, set_impl_nat)
           (fvi zero_nata (Eq (Div (vb, vc), va))) &&
           mmonitorable_exec (Eq (Div (vb, vc), va))
     | Neg (Eq (Mod (vb, vc), va)) ->
-        is_empty (card_UNIV_nat, ceq_nat, cproper_interval_nat)
+        is_empty (card_UNIV_nat, ceq_nat, cproper_interval_nat, set_impl_nat)
           (fvi zero_nata (Eq (Mod (vb, vc), va))) &&
           mmonitorable_exec (Eq (Mod (vb, vc), va))
     | Neg (Eq (F2i vb, va)) ->
-        is_empty (card_UNIV_nat, ceq_nat, cproper_interval_nat)
+        is_empty (card_UNIV_nat, ceq_nat, cproper_interval_nat, set_impl_nat)
           (fvi zero_nata (Eq (F2i vb, va))) &&
           mmonitorable_exec (Eq (F2i vb, va))
     | Neg (Eq (I2f vb, va)) ->
-        is_empty (card_UNIV_nat, ceq_nat, cproper_interval_nat)
+        is_empty (card_UNIV_nat, ceq_nat, cproper_interval_nat, set_impl_nat)
           (fvi zero_nata (Eq (I2f vb, va))) &&
           mmonitorable_exec (Eq (I2f vb, va))
     | Neg (Eq (v, Const vb)) ->
-        is_empty (card_UNIV_nat, ceq_nat, cproper_interval_nat)
+        is_empty (card_UNIV_nat, ceq_nat, cproper_interval_nat, set_impl_nat)
           (fvi zero_nata (Eq (v, Const vb))) &&
           mmonitorable_exec (Eq (v, Const vb))
     | Neg (Eq (v, Plus (vb, vc))) ->
-        is_empty (card_UNIV_nat, ceq_nat, cproper_interval_nat)
+        is_empty (card_UNIV_nat, ceq_nat, cproper_interval_nat, set_impl_nat)
           (fvi zero_nata (Eq (v, Plus (vb, vc)))) &&
           mmonitorable_exec (Eq (v, Plus (vb, vc)))
     | Neg (Eq (v, Minus (vb, vc))) ->
-        is_empty (card_UNIV_nat, ceq_nat, cproper_interval_nat)
+        is_empty (card_UNIV_nat, ceq_nat, cproper_interval_nat, set_impl_nat)
           (fvi zero_nata (Eq (v, Minus (vb, vc)))) &&
           mmonitorable_exec (Eq (v, Minus (vb, vc)))
     | Neg (Eq (v, UMinus vb)) ->
-        is_empty (card_UNIV_nat, ceq_nat, cproper_interval_nat)
+        is_empty (card_UNIV_nat, ceq_nat, cproper_interval_nat, set_impl_nat)
           (fvi zero_nata (Eq (v, UMinus vb))) &&
           mmonitorable_exec (Eq (v, UMinus vb))
     | Neg (Eq (v, Mult (vb, vc))) ->
-        is_empty (card_UNIV_nat, ceq_nat, cproper_interval_nat)
+        is_empty (card_UNIV_nat, ceq_nat, cproper_interval_nat, set_impl_nat)
           (fvi zero_nata (Eq (v, Mult (vb, vc)))) &&
           mmonitorable_exec (Eq (v, Mult (vb, vc)))
     | Neg (Eq (v, Div (vb, vc))) ->
-        is_empty (card_UNIV_nat, ceq_nat, cproper_interval_nat)
+        is_empty (card_UNIV_nat, ceq_nat, cproper_interval_nat, set_impl_nat)
           (fvi zero_nata (Eq (v, Div (vb, vc)))) &&
           mmonitorable_exec (Eq (v, Div (vb, vc)))
     | Neg (Eq (v, Mod (vb, vc))) ->
-        is_empty (card_UNIV_nat, ceq_nat, cproper_interval_nat)
+        is_empty (card_UNIV_nat, ceq_nat, cproper_interval_nat, set_impl_nat)
           (fvi zero_nata (Eq (v, Mod (vb, vc)))) &&
           mmonitorable_exec (Eq (v, Mod (vb, vc)))
     | Neg (Eq (v, F2i vb)) ->
-        is_empty (card_UNIV_nat, ceq_nat, cproper_interval_nat)
+        is_empty (card_UNIV_nat, ceq_nat, cproper_interval_nat, set_impl_nat)
           (fvi zero_nata (Eq (v, F2i vb))) &&
           mmonitorable_exec (Eq (v, F2i vb))
     | Neg (Eq (v, I2f vb)) ->
-        is_empty (card_UNIV_nat, ceq_nat, cproper_interval_nat)
+        is_empty (card_UNIV_nat, ceq_nat, cproper_interval_nat, set_impl_nat)
           (fvi zero_nata (Eq (v, I2f vb))) &&
           mmonitorable_exec (Eq (v, I2f vb))
     | Neg (Less (v, va)) ->
-        is_empty (card_UNIV_nat, ceq_nat, cproper_interval_nat)
+        is_empty (card_UNIV_nat, ceq_nat, cproper_interval_nat, set_impl_nat)
           (fvi zero_nata (Less (v, va))) &&
           mmonitorable_exec (Less (v, va))
     | Neg (LessEq (v, va)) ->
-        is_empty (card_UNIV_nat, ceq_nat, cproper_interval_nat)
+        is_empty (card_UNIV_nat, ceq_nat, cproper_interval_nat, set_impl_nat)
           (fvi zero_nata (LessEq (v, va))) &&
           mmonitorable_exec (LessEq (v, va))
     | Neg (Neg v) ->
-        is_empty (card_UNIV_nat, ceq_nat, cproper_interval_nat)
+        is_empty (card_UNIV_nat, ceq_nat, cproper_interval_nat, set_impl_nat)
           (fvi zero_nata (Neg v)) &&
           mmonitorable_exec (Neg v)
     | Neg (Or (v, va)) ->
-        is_empty (card_UNIV_nat, ceq_nat, cproper_interval_nat)
+        is_empty (card_UNIV_nat, ceq_nat, cproper_interval_nat, set_impl_nat)
           (fvi zero_nata (Or (v, va))) &&
           mmonitorable_exec (Or (v, va))
     | Neg (And (v, va)) ->
-        is_empty (card_UNIV_nat, ceq_nat, cproper_interval_nat)
+        is_empty (card_UNIV_nat, ceq_nat, cproper_interval_nat, set_impl_nat)
           (fvi zero_nata (And (v, va))) &&
           mmonitorable_exec (And (v, va))
     | Neg (Ands v) ->
-        is_empty (card_UNIV_nat, ceq_nat, cproper_interval_nat)
+        is_empty (card_UNIV_nat, ceq_nat, cproper_interval_nat, set_impl_nat)
           (fvi zero_nata (Ands v)) &&
           mmonitorable_exec (Ands v)
     | Neg (Exists v) ->
-        is_empty (card_UNIV_nat, ceq_nat, cproper_interval_nat)
+        is_empty (card_UNIV_nat, ceq_nat, cproper_interval_nat, set_impl_nat)
           (fvi zero_nata (Exists v)) &&
           mmonitorable_exec (Exists v)
     | Neg (Agg (v, va, vb, vc, vd)) ->
-        is_empty (card_UNIV_nat, ceq_nat, cproper_interval_nat)
+        is_empty (card_UNIV_nat, ceq_nat, cproper_interval_nat, set_impl_nat)
           (fvi zero_nata (Agg (v, va, vb, vc, vd))) &&
           mmonitorable_exec (Agg (v, va, vb, vc, vd))
     | Neg (Prev (v, va)) ->
-        is_empty (card_UNIV_nat, ceq_nat, cproper_interval_nat)
+        is_empty (card_UNIV_nat, ceq_nat, cproper_interval_nat, set_impl_nat)
           (fvi zero_nata (Prev (v, va))) &&
           mmonitorable_exec (Prev (v, va))
     | Neg (Next (v, va)) ->
-        is_empty (card_UNIV_nat, ceq_nat, cproper_interval_nat)
+        is_empty (card_UNIV_nat, ceq_nat, cproper_interval_nat, set_impl_nat)
           (fvi zero_nata (Next (v, va))) &&
           mmonitorable_exec (Next (v, va))
     | Neg (Since (v, va, vb)) ->
-        is_empty (card_UNIV_nat, ceq_nat, cproper_interval_nat)
+        is_empty (card_UNIV_nat, ceq_nat, cproper_interval_nat, set_impl_nat)
           (fvi zero_nata (Since (v, va, vb))) &&
           mmonitorable_exec (Since (v, va, vb))
     | Neg (Until (v, va, vb)) ->
-        is_empty (card_UNIV_nat, ceq_nat, cproper_interval_nat)
+        is_empty (card_UNIV_nat, ceq_nat, cproper_interval_nat, set_impl_nat)
           (fvi zero_nata (Until (v, va, vb))) &&
           mmonitorable_exec (Until (v, va, vb))
     | Neg (Trigger (v, va, vb)) ->
-        is_empty (card_UNIV_nat, ceq_nat, cproper_interval_nat)
+        is_empty (card_UNIV_nat, ceq_nat, cproper_interval_nat, set_impl_nat)
           (fvi zero_nata (Trigger (v, va, vb))) &&
           mmonitorable_exec (Trigger (v, va, vb))
     | Neg (Release (v, va, vb)) ->
-        is_empty (card_UNIV_nat, ceq_nat, cproper_interval_nat)
+        is_empty (card_UNIV_nat, ceq_nat, cproper_interval_nat, set_impl_nat)
           (fvi zero_nata (Release (v, va, vb))) &&
           mmonitorable_exec (Release (v, va, vb))
     | Neg (MatchF (v, va)) ->
-        is_empty (card_UNIV_nat, ceq_nat, cproper_interval_nat)
+        is_empty (card_UNIV_nat, ceq_nat, cproper_interval_nat, set_impl_nat)
           (fvi zero_nata (MatchF (v, va))) &&
           mmonitorable_exec (MatchF (v, va))
     | Neg (MatchP (v, va)) ->
-        is_empty (card_UNIV_nat, ceq_nat, cproper_interval_nat)
+        is_empty (card_UNIV_nat, ceq_nat, cproper_interval_nat, set_impl_nat)
           (fvi zero_nata (MatchP (v, va))) &&
           mmonitorable_exec (MatchP (v, va))
     | Or (phi, psi) ->
@@ -8943,8 +9000,18 @@ let rec mmonitorable_exec
                     | Since (_, _, _) -> false | Until (_, _, _) -> false
                     | Trigger (a, b, c) ->
                       safe_formula_dual true mmonitorable_exec a b c
-                    | Release (_, _, _) -> false | MatchF (_, _) -> false
-                    | MatchP (_, _) -> false))))
+                    | Release (phia, i, psia) ->
+                      bounded i &&
+                        (not (memL i zero_nata && memR i zero_nata) &&
+                          (mmonitorable_exec phia &&
+                            (mmonitorable_exec psia &&
+                              (eq_set
+                                 (card_UNIV_nat, cenum_nat, ceq_nat,
+                                   ccompare_nat)
+                                 (fvi zero_nata phia) (fvi zero_nata psia) &&
+                                mmonitorable_exec
+                                  (and_release_safe_bounded phi phia i psia)))))
+                    | MatchF (_, _) -> false | MatchP (_, _) -> false))))
     | Ands l ->
         (let (pos, neg) = partition mmonitorable_exec l in
           not (null pos) &&
@@ -9120,8 +9187,20 @@ let rec convert_multiway
                                    | MatchP (_, _) -> false)
                                then And (convert_multiway phi,
   convert_multiway psi)
-                               else Ands (convert_multiway psi ::
-   get_and_list (convert_multiway phi))))))
+                               else (if (match psi with Pred (_, _) -> false
+  | Let (_, _, _) -> false | Eq (_, _) -> false | Less (_, _) -> false
+  | LessEq (_, _) -> false | Neg _ -> false | Or (_, _) -> false
+  | And (_, _) -> false | Ands _ -> false | Exists _ -> false
+  | Agg (_, _, _, _, _) -> false | Prev (_, _) -> false | Next (_, _) -> false
+  | Since (_, _, _) -> false | Until (_, _, _) -> false
+  | Trigger (_, _, _) -> false | Release (_, _, _) -> true
+  | MatchF (_, _) -> false | MatchP (_, _) -> false)
+                                      then (let Release (phia, i, psia) = psi in
+     (if memL i zero_nata && memR i zero_nata
+       then And (convert_multiway phi, convert_multiway psi)
+       else convert_multiway (and_release_safe_bounded phi phia i psia)))
+                                      else Ands
+     (convert_multiway psi :: get_and_list (convert_multiway phi)))))))
     | Ands phi_s -> Ands (mapa convert_multiway phi_s)
     | Exists phi -> Exists (convert_multiway phi)
     | Agg (y, omega, b, f, phi) -> Agg (y, omega, b, f, convert_multiway phi)
@@ -9133,11 +9212,102 @@ let rec convert_multiway
         Until (convert_multiway phi, i, convert_multiway psi)
     | Trigger (phi, i, psi) ->
         Trigger (convert_multiway phi, i, convert_multiway psi)
-    | Release (phi, i, psi) -> convert_multiway (release_safe_0 phi i psi)
+    | Release (phi, i, psi) ->
+        (if memL i zero_nata && memR i zero_nata
+          then convert_multiway (release_safe_0 phi i psi)
+          else convert_multiway (release_safe_bounded phi i psi))
     | MatchP (i, r) -> MatchP (i, map_regex convert_multiway r)
     | MatchF (i, r) -> MatchF (i, map_regex convert_multiway r);;
 
 let rec vminit_safe
   phi = (if mmonitorable_exec phi then vminit phi else failwith "undefined");;
+
+let rec historically_safe_bounded
+  i phi =
+    And (once i phi,
+          Neg (once i
+                (And (Or (once (int_remove_lower_bound i) phi,
+                           eventually (int_remove_lower_bound i) phi),
+                       Neg phi))));;
+
+let rec trigger_safe_bounded
+  phi i psi =
+    And (once i tt,
+          Or (Or (historically_safe_bounded i psi,
+                   once (flip_int_less_lower i) phi),
+               once (flip_int_less_lower i)
+                 (Prev (all, Since (psi, int_remove_lower_bound i,
+                                     And (phi, psi))))));;
+
+let rec historically_safe_unbounded
+  i phi =
+    And (once (flip_int_less_lower i)
+           (Prev (all, Since (phi, all, And (phi, first)))),
+          once i phi);;
+
+let rec trigger_safe_unbounded
+  phi i psi =
+    And (once i tt,
+          Or (Or (historically_safe_unbounded i psi,
+                   once (flip_int_less_lower i) phi),
+               once (flip_int_less_lower i)
+                 (Prev (all, Since (psi, int_remove_lower_bound i,
+                                     And (phi, psi))))));;
+
+let rec and_trigger_safe_bounded
+  phia phi i psi =
+    Or (And (phia, Neg (once i tt)),
+         And (phia, trigger_safe_bounded phi i psi));;
+
+let rec and_trigger_safe_unbounded
+  phia phi i psi =
+    Or (And (phia, Neg (once i tt)),
+         And (phia, trigger_safe_unbounded phi i psi));;
+
+let rec rewrite_trigger
+  = function
+    And (phi, Trigger (alpha, i, beta)) ->
+      (if memL i zero_nata && memR i zero_nata
+        then And (phi, Trigger (alpha, i, beta))
+        else (if bounded i then and_trigger_safe_bounded phi alpha i beta
+               else and_trigger_safe_unbounded phi alpha i beta))
+    | Trigger (alpha, i, beta) ->
+        (if memL i zero_nata && memR i zero_nata
+          then trigger_safe_0 alpha i beta else Trigger (alpha, i, beta))
+    | Pred (v, va) -> Pred (v, va)
+    | Let (v, va, vb) -> Let (v, va, vb)
+    | Eq (v, va) -> Eq (v, va)
+    | Less (v, va) -> Less (v, va)
+    | LessEq (v, va) -> LessEq (v, va)
+    | Neg v -> Neg v
+    | Or (v, va) -> Or (v, va)
+    | And (v, Pred (vb, vc)) -> And (v, Pred (vb, vc))
+    | And (v, Let (vb, vc, vd)) -> And (v, Let (vb, vc, vd))
+    | And (v, Eq (vb, vc)) -> And (v, Eq (vb, vc))
+    | And (v, Less (vb, vc)) -> And (v, Less (vb, vc))
+    | And (v, LessEq (vb, vc)) -> And (v, LessEq (vb, vc))
+    | And (v, Neg vb) -> And (v, Neg vb)
+    | And (v, Or (vb, vc)) -> And (v, Or (vb, vc))
+    | And (v, And (vb, vc)) -> And (v, And (vb, vc))
+    | And (v, Ands vb) -> And (v, Ands vb)
+    | And (v, Exists vb) -> And (v, Exists vb)
+    | And (v, Agg (vb, vc, vd, ve, vf)) -> And (v, Agg (vb, vc, vd, ve, vf))
+    | And (v, Prev (vb, vc)) -> And (v, Prev (vb, vc))
+    | And (v, Next (vb, vc)) -> And (v, Next (vb, vc))
+    | And (v, Since (vb, vc, vd)) -> And (v, Since (vb, vc, vd))
+    | And (v, Until (vb, vc, vd)) -> And (v, Until (vb, vc, vd))
+    | And (v, Release (vb, vc, vd)) -> And (v, Release (vb, vc, vd))
+    | And (v, MatchF (vb, vc)) -> And (v, MatchF (vb, vc))
+    | And (v, MatchP (vb, vc)) -> And (v, MatchP (vb, vc))
+    | Ands v -> Ands v
+    | Exists v -> Exists v
+    | Agg (v, va, vb, vc, vd) -> Agg (v, va, vb, vc, vd)
+    | Prev (v, va) -> Prev (v, va)
+    | Next (v, va) -> Next (v, va)
+    | Since (v, va, vb) -> Since (v, va, vb)
+    | Until (v, va, vb) -> Until (v, va, vb)
+    | Release (v, va, vb) -> Release (v, va, vb)
+    | MatchF (v, va) -> MatchF (v, va)
+    | MatchP (v, va) -> MatchP (v, va);;
 
 end;; (*struct Monitor*)
